verify erpc.Client__NewRequest

external/Goose/github_com/mit_pdos/gokv/erpc.v
@@ -55,15 +55,16 @@ Definition MakeServer: val :=
 
 Definition Client := struct.decl [
   "cid" :: uint64T;
-  "seq" :: uint64T
+  "nextSeq" :: uint64T
 ].
 
 Definition Client__NewRequest: val :=
   rec: "Client__NewRequest" "c" "request" :=
-    struct.storeF Client "seq" "c" (std.SumAssumeNoOverflow (struct.loadF Client "seq" "c") #1);;
+    let: "seq" := struct.loadF Client "nextSeq" "c" in
+    struct.storeF Client "nextSeq" "c" (std.SumAssumeNoOverflow (struct.loadF Client "nextSeq" "c") #1);;
     let: "data1" := NewSliceWithCap byteT #0 (#8 + #8 + slice.len "request") in
     let: "data2" := marshal.WriteInt "data1" (struct.loadF Client "cid" "c") in
-    let: "data3" := marshal.WriteInt "data2" (struct.loadF Client "seq" "c") in
+    let: "data3" := marshal.WriteInt "data2" "seq" in
     let: "data4" := marshal.WriteBytes "data3" "request" in
     "data4".
 
@@ -71,7 +72,7 @@ Definition MakeClient: val :=
   rec: "MakeClient" "cid" :=
     let: "c" := struct.alloc Client (zero_val (struct.t Client)) in
     struct.storeF Client "cid" "c" "cid";;
-    struct.storeF Client "seq" "c" #0;;
+    struct.storeF Client "nextSeq" "c" #1;;
     "c".
 
 End code.
